ulib: tactics: consistent thunking
lot of TODOs and weird behaviours

also move some tactic code from
examples/tactics/micro-benchmarks/UserTactics.Example1.fst into
FStar.Tactics.fst.

ulib/FStar.Tactics.fst
@@ -34,21 +34,23 @@ noeq type formula =
   //Abs   : binders -> term -> formula //Named repr
   //Match : ....
 
-noeq type result (a:Type) =
-  | Success: a -> state -> result a
-  | Failed: string -> state -> result a
+noeq type _result (a:Type) =
+  | Success: a -> state -> _result a
+  | Failed: string -> state -> _result a
 
-let tac (a:Type) = state -> M (result a)
+(* If it starts with an underline don't use it from the outside! *)
+
+let _tac (a:Type) = state -> M (_result a)
 
 (* monadic return *)
-val ret : a:Type -> x:a -> tac a
-let ret a x = fun (s:state) -> Success x s
+val _ret : a:Type -> x:a -> _tac a
+let _ret a x = fun (s:state) -> Success x s
 
 (* monadic bind *)
-let bind (a:Type) (b:Type) 
-         (t1:tac a)
-         (t2:a -> tac b)
-    : tac b
+let _bind (a:Type) (b:Type) 
+         (t1:_tac a)
+         (t2:a -> _tac b)
+    : _tac b
     = fun p ->
         let r = t1 p in
         match r with
@@ -56,36 +58,39 @@ let bind (a:Type) (b:Type)
         | Failed msg q -> Failed msg q
 
 (* Actions *)
-let get () : tac state = fun s0 -> Success s0 s0 
+let _get () : _tac state = fun s0 -> Success s0 s0 
 
 
 (* total  *) //disable the termination check, although it remains reifiable
 reifiable reflectable new_effect {
   TAC : a:Type -> Effect
-  with repr     = tac
-     ; bind     = bind
-     ; return   = ret
-     ; get      = get
+  with repr     = _tac
+     ; bind     = _bind
+     ; return   = _ret
+     ; _get     = _get
 }
 effect Tac (a:Type) = TAC a (fun i post -> forall j. post j)
 let tactic (a:Type) = unit -> Tac a
 
 (* working around #885 *)
-let fail_ (a:Type) (msg:string) : tac a = fun s0 -> Failed #a msg s0
-let fail (#a:Type) (msg:string) = TAC?.reflect (fail_ a msg)
+let _fail (a:Type) (msg:string) : _tac a = fun s0 -> Failed #a msg s0
+let fail (#a:Type) (msg:string) : tactic a = fun () -> TAC?.reflect (_fail a msg)
 
 let or_else (#a:Type) (t1:tactic a) (t2:tactic a)
-        : Tac a
-        = TAC?.reflect (fun p -> 
+        : tactic a
+        = fun () ->
+          TAC?.reflect (fun p -> 
             match reify (t1 ()) p with
-            | Failed _ _ -> 
-              reify (t2 ()) p
-              | q -> q)
+            | Failed _ _ -> reify (t2 ()) p
+            | q -> q)
 
+// TODO: forgot the underscore in result and F* blew up,
+// didn't mention a undefined "result". bug?
 abstract 
-let by_tactic (t:state -> result unit) (a:Type) : Type = a
+let by_tactic (t:state -> _result unit) (a:Type) : Type = a
 
-let reify_tactic (t:tactic unit) : tac unit =
+// TODO: generalize to any type
+let reify_tactic (t:tactic unit) : _tac unit =
   fun s -> reify (t ()) s
 
 let assert_by_tactic (t:tactic unit) (p:Type)
@@ -94,14 +99,16 @@ let assert_by_tactic (t:tactic unit) (p:Type)
          (ensures (fun _ -> p))
   = ()
 
+  // TODO: naming convention.. underscore before or after?
+
 assume private val binders_of_env_ : env -> binders
-let binders_of_env (e:env) : Tac binders = binders_of_env_ e
+let binders_of_env (e:env) : tactic binders = fun () -> binders_of_env_ e
 
 assume private val type_of_binder_: binder -> term 
-let type_of_binder (b:binder) : Tac term = type_of_binder_ b
+let type_of_binder (b:binder) : tactic term = fun () -> type_of_binder_ b
 
 assume private val term_eq_ : term -> term -> bool
-let term_eq t1 t2 : Tac bool = term_eq_ t1 t2
+let term_eq t1 t2 : tactic bool = fun () ->  term_eq_ t1 t2
 
 assume private val embed  : #a:Type -> a -> term
 let quote #a (x:a) : tactic term = fun () -> embed x
@@ -109,59 +116,217 @@ let quote #a (x:a) : tactic term = fun () -> embed x
 //This primitive provides a way to destruct a term as a formula
 //TODO: We should add a formula_as_term also
 assume private val term_as_formula_ : term -> option formula
-let term_as_formula t : Tac (option formula) = term_as_formula_ t
+let term_as_formula t : tactic (option formula) = fun () -> term_as_formula_ t
 
 (* Many of these could be derived from apply_lemma, 
    rather than being assumed as primitives. 
    E.g., forall_intros could be an application of 
          FStar.Classical.forall_intro
  *)         
-assume private val forall_intros_: tac binders
-let forall_intros () : Tac binders = TAC?.reflect forall_intros_
+assume private val forall_intros_: _tac binders
+let forall_intros : tactic binders = fun () -> TAC?.reflect forall_intros_
 
-assume private val implies_intro_: tac binder
-let implies_intro () : Tac binder = TAC?.reflect implies_intro_
+assume private val implies_intro_: _tac binder
+let implies_intro : tactic binder = fun () -> TAC?.reflect implies_intro_
 
-assume private val trivial_  : tac unit
-let trivial () : Tac unit = TAC?.reflect trivial_
+assume private val trivial_  : _tac unit
+let trivial : tactic unit = fun () -> TAC?.reflect trivial_
 
-assume private val revert_  : tac unit
-let revert () : Tac unit = TAC?.reflect revert_
+assume private val revert_  : _tac unit
+let revert : tactic unit = fun () -> TAC?.reflect revert_
 
-assume private val clear_   : tac unit
-let clear () : Tac unit = TAC?.reflect clear_
+assume private val clear_   : _tac unit
+let clear : tactic unit = fun () -> TAC?.reflect clear_
 
-assume private val split_   : tac unit
-let split () : Tac unit = TAC?.reflect split_
+assume private val split_   : _tac unit
+let split : tactic unit = fun () -> TAC?.reflect split_
 
-assume private val merge_   : tac unit
-let merge () : Tac unit = TAC?.reflect merge_
+assume private val merge_   : _tac unit
+let merge : tactic unit = fun () -> TAC?.reflect merge_
 
-assume private val rewrite_ : binder -> tac unit
-let rewrite (b:binder) : Tac unit = TAC?.reflect (rewrite_ b)
+assume private val rewrite_ : binder -> _tac unit
+let rewrite (b:binder) : tactic unit = fun () -> TAC?.reflect (rewrite_ b)
 
-assume private val smt_     : tac unit
-let smt () : Tac unit = TAC?.reflect smt_
+assume private val smt_     : _tac unit
+let smt : tactic unit = fun () -> TAC?.reflect smt_
 
-assume private val visit_   : tac unit -> tac unit
-let visit (f:tactic unit) : Tac unit = TAC?.reflect (visit_ (reify_tactic f))
+assume private val visit_   : _tac unit -> _tac unit
+let visit (f:tactic unit) : tactic unit = fun () -> TAC?.reflect (visit_ (reify_tactic f))
 
-assume private val focus_: tac unit -> tac unit
-let focus (f:tactic unit) : Tac unit = TAC?.reflect (focus_ (reify_tactic f))
+assume private val focus_: _tac unit -> _tac unit
+let focus (f:tactic unit) : tactic unit = fun () -> TAC?.reflect (focus_ (reify_tactic f))
 
 (* could be implemented using focus_ *)
-assume private val seq_ : tac unit -> tac unit -> tac unit
+assume private val seq_ : _tac unit -> _tac unit -> _tac unit
 let seq (f:tactic unit) (g:tactic unit) : tactic unit = fun () -> 
   TAC?.reflect (seq_ (reify_tactic f) (reify_tactic g))
 
-assume private val exact_ : term -> tac unit
-let exact (t:term) : Tac unit = TAC?.reflect (exact_ t)
+assume private val exact_ : term -> _tac unit
+let exact (t:term) : tactic unit = fun () -> TAC?.reflect (exact_ t)
 
-assume private val apply_lemma_ : term -> tac unit
-let apply_lemma (t:term) : Tac unit = TAC?.reflect (apply_lemma_ t)
+assume private val apply_lemma_ : term -> _tac unit
+let apply_lemma (t:term) : tactic unit = fun () -> TAC?.reflect (apply_lemma_ t)
 
-assume val print_ : string -> tac unit
-let print (msg:string) : Tac unit = TAC?.reflect (print_ msg)
+assume val print_ : string -> _tac unit
+let print (msg:string) : tactic unit = fun () -> TAC?.reflect (print_ msg)
 
-assume val grewrite_ : term -> term -> tac unit
-let grewrite (e1:term) (e2:term) : Tac unit = TAC?.reflect (grewrite_ e1 e2)
+assume val grewrite_ : term -> term -> _tac unit
+let grewrite (e1:term) (e2:term) : tactic unit = fun () -> TAC?.reflect (grewrite_ e1 e2)
+
+// For some reason, a direct definition fails.
+let revert_all (bs:binders) : tactic unit =
+    let rec _revert_all (bs:binders) : Tac unit =
+      match bs with
+      | [] -> ()
+      | _::tl -> let _ = revert () in _revert_all tl
+    in fun () -> _revert_all bs
+
+let get : tactic state = fun () -> TAC?._get ()
+
+let cur_goal : tactic goal = fun () ->
+  let goals, _ = get () in
+  match goals with
+  | [] -> fail "No more goals" ()
+  | hd::_ -> hd
+
+let destruct_equality_implication (t:term) : tactic (option (formula * term)) = fun () ->
+  match term_as_formula t () with
+  | Some (Implies lhs rhs) ->
+    let lhs = term_as_formula lhs () in
+    (match lhs with
+     | Some (Eq _ _ _) -> Some (Some?.v lhs, rhs)
+     | _ -> None)
+  | _ -> None
+
+// TODO: Needs to be unit -> Tac unit since it's a let rec.
+let rec simplify_eq_implication : unit -> Tac unit
+  = fun () ->
+    let context, goal_t = cur_goal () in  // G |- x=e ==> P
+    match destruct_equality_implication goal_t () with
+    | None -> fail "Not an equality implication" ()
+    | Some (_, rhs) ->
+      let eq_h = implies_intro () in  // G, eq_h:x=e |- P
+      rewrite eq_h (); // G, eq_h:x=e |- P[e/x]
+      clear ();     // G |- P[e/x]
+      visit simplify_eq_implication ()
+
+// TODO: aux isn't used. wtf?
+// in this one, if the return type is "tactic unit", it complains
+// about not being able to show a decreasing order. again wtf?
+let rec user_visit (callback:tactic unit) : unit -> Tac unit
+    = fun () ->
+         let aux : tactic unit = fun () ->
+           let context, goal_t = cur_goal () in
+           match term_as_formula goal_t () with
+           | None -> smt ()
+           | Some (Exists _ _) -> //not yet handled
+             ()
+
+           | Some (Forall xs body) ->
+             let binders = forall_intros () in
+             let _ = user_visit callback () in
+             revert_all binders ()
+
+           | Some (And t1 t2) ->
+             let _ = seq split (user_visit callback) () in
+             merge ()
+
+           | Some (Implies t1 t2) ->
+             let h = implies_intro () in
+             let _ = user_visit callback () in
+             revert ()
+
+           | _ ->
+             or_else trivial smt ()
+         in
+         or_else callback (user_visit callback) ()
+
+let rec try_rewrite_equality (x:term)
+                             (bs:binders)
+  : tactic unit
+  = fun () ->
+    match bs with
+    | [] -> ()
+    | x_t::bs -> begin
+      match term_as_formula (type_of_binder x_t ()) () with
+      | Some (Eq _ y _) ->
+        if term_eq x y ()
+        then rewrite x_t ()
+        else try_rewrite_equality x bs ()
+      | _ -> try_rewrite_equality x bs ()
+      end
+
+let rec rewrite_all_context_equalities (bs:binders)
+  : tactic unit
+  = fun () ->
+    match bs with
+    | [] -> ()
+    | x_t::bs -> begin
+      match term_as_formula (type_of_binder x_t ()) () with
+      | Some (Eq _ _ _) ->
+        rewrite x_t ();
+        rewrite_all_context_equalities bs ()
+      | _ ->
+        rewrite_all_context_equalities bs ()
+      end
+
+// TODO: has to be arrow
+let rec rewrite_eqs_from_context : unit -> Tac unit
+  = fun () ->
+       let context, _ = cur_goal () in
+       rewrite_all_context_equalities (binders_of_env context ()) ()
+
+let rewrite_equality (x:tactic term) : tactic unit
+  = fun () ->
+     let context, _ = cur_goal () in
+     try_rewrite_equality (x ()) (binders_of_env context ()) ()
+
+let solved : tactic unit = fun () ->
+  let _, goal = cur_goal () in
+  match term_as_formula goal () with
+  | Some True_ -> ()
+  | _ -> fail "Not solved" ()
+
+let rec just_do_intros : unit -> Tac unit =
+    focus (fun () ->
+       let _ = forall_intros () in
+       let _ = implies_intro () in
+       smt ();
+       revert ();
+       revert ())
+
+// TODO: again has to be an arrow
+let rec rewrite_all_equalities : unit -> Tac unit = fun () ->
+  visit simplify_eq_implication ()
+
+
+assume val lemma_mul_comm : x:nat -> y:nat -> Lemma (op_Multiply x y == op_Multiply y x)
+let mul_commute_ascription : tactic unit
+  = fun () ->
+    let _, goal_t = cur_goal () in  // G |- x=e ==> P
+    match term_as_formula goal_t () with
+    | Some (Eq _ _ _) ->
+      apply_lemma (quote lemma_mul_comm ()) ()
+    | _ -> fail "Not an equality" ()
+
+// TODO: unfold tactic or complains about termination
+let rec unfold_definition_and_simplify_eq' (tm:term)
+  : unit -> Tac unit
+  = fun () ->
+      let _, goal_t = cur_goal () in  // G |- x=e ==> P
+      match term_as_formula goal_t () with
+      | Some (App hd arg) ->
+        if term_eq hd tm () then trivial ()
+      | _ -> begin
+        match destruct_equality_implication goal_t () with
+        | None -> fail "Not an equality implication" ()
+        | Some (_, rhs) ->
+          let eq_h = implies_intro () in  // G, eq_h:x=e |- P
+          rewrite eq_h (); // G, eq_h:x=e |- P[e/x]
+          clear ();     // G |- P[e/x]
+          visit (unfold_definition_and_simplify_eq' tm) ()
+       end
+
+let unfold_definition_and_simplify_eq (tm:tactic term) 
+  : tactic unit 
+  = fun () -> unfold_definition_and_simplify_eq' (tm ()) ()
